prettify saved_prop interface: hide the Next

program_logic/saved_prop.v
@@ -4,18 +4,18 @@ Import uPred.
 
 Class savedPropG (Λ : language) (Σ : gFunctors) (F : cFunctor) :=
   SavedPropG {
-    saved_prop_F_contractive :> cFunctorContractive F;
-    saved_prop_inG :> inG Λ Σ (agreeR (F (iPreProp Λ (globalF Σ))));
+    saved_prop_F_contractive :> cFunctorNe F;
+    saved_prop_inG :> inG Λ Σ (agreeR $ laterC (F (iPreProp Λ (globalF Σ))));
   }.
-Definition savedPropGF (F : cFunctor) `{cFunctorContractive F} :
-  gFunctor := GFunctor (agreeRF F).
-Instance inGF_savedPropG `{cFunctorContractive F}
+Definition savedPropGF (F : cFunctor) `{cFunctorNe F} :
+  gFunctor := GFunctor (agreeRF $ laterCF F).
+Instance inGF_savedPropG `{cFunctorNe F}
          `{inGF Λ Σ (savedPropGF F)} : savedPropG Λ Σ F.
 Proof. split; try apply _; apply: inGF_inG. Qed.
 
 Definition saved_prop_own `{savedPropG Λ Σ F}
     (γ : gname) (x : F (iPropG Λ Σ)) : iPropG Λ Σ :=
-  own γ (to_agree (cFunctor_map F (iProp_fold, iProp_unfold) x)).
+  own γ (to_agree $ Next (cFunctor_map F (iProp_fold, iProp_unfold) x)).
 Typeclasses Opaque saved_prop_own.
 Instance: Params (@saved_prop_own) 4.
 
@@ -36,16 +36,16 @@ Section saved_prop.
   Proof. by apply own_alloc. Qed.
 
   Lemma saved_prop_agree γ x y :
-    (saved_prop_own γ x ★ saved_prop_own γ y) ⊑ (x ≡ y).
+    (saved_prop_own γ x ★ saved_prop_own γ y) ⊑ ▷(x ≡ y).
   Proof.
-    rewrite -own_op own_valid agree_validI agree_equivI.
+    rewrite -own_op own_valid agree_validI agree_equivI later_equivI.
     set (G1 := cFunctor_map F (iProp_fold, iProp_unfold)).
     set (G2 := cFunctor_map F (@iProp_unfold Λ (globalF Σ),
                                @iProp_fold Λ (globalF Σ))).
     assert (∀ z, G2 (G1 z) ≡ z) as help.
     { intros z. rewrite /G1 /G2 -cFunctor_compose -{2}[z]cFunctor_id.
       apply (ne_proper (cFunctor_map F)); split=>?; apply iProp_fold_unfold. }
-    rewrite -{2}[x]help -{2}[y]help.
+    rewrite -{2}[x]help -{2}[y]help. apply later_mono.
     apply (eq_rewrite (G1 x) (G1 y) (λ z, G2 (G1 x) ≡ G2 z))%I;
       first solve_proper; auto with I.
   Qed.
